checkpoint
@kha I tried to implement string as (array char), unfortunately I hit
many bootstrapping problems. The main issue is that basic string
operations (e.g., equality and concatenation) need similar operations
for arrays, and the array operations need arithmetic lemmas to prove
that the positions being read are inside the array bounds.
However, most of these lemmas are proved using the tactic framework,
and the tactic framework requires strings :(
I managed to implement the decidable equality for array and string
without significant overhead. However, array/string append (and other
operations) will be very inefficient when we stop using persistent
arrays. Actually even with persistent arrays I noticed performance problems.
To make things more complicated, the string implementation is sealed,
and the internals can only be accessed at init/data/string/basic.lean.

String slicing operations will also be very inefficient if we don't
use the array slice function that currently depends on the tactic framework.

Right now, I'm inclined to keep string as a list of char, and use
char_buffer for parsing.

Any thoughts?

src/library/vm/vm_string.cpp
@@ -6,14 +6,16 @@ Author: Leonardo de Moura
 */
 #include <string>
 #include "util/interrupt.h"
+#include "library/parray.h"
 #include "library/vm/vm_string.h"
+#include "library/vm/vm_array.h"
 
 namespace lean {
 static void to_string(vm_obj const & o, std::string & s) {
     check_system("to_string");
-    if (!is_simple(o)) {
-        to_string(cfield(o, 1), s);
-        s += static_cast<unsigned char>(cidx(cfield(o, 0)));
+    parray<vm_obj> const & a = to_array(cfield(o, 1));
+    for (size_t i = 0; i < a.size(); i++) {
+        s += static_cast<unsigned char>(cidx(a[i]));
     }
 }
 
@@ -24,11 +26,10 @@ std::string to_string(vm_obj const & o) {
 }
 
 vm_obj to_obj(std::string const & str) {
-    vm_obj r = mk_vm_simple(0);
-    for (unsigned i = 0; i < str.size(); i++) {
-        vm_obj args[2] = { mk_vm_simple(static_cast<unsigned char>(str[i])), r };
-        r = mk_vm_constructor(1, 2, args);
+    parray<vm_obj> a;
+    for (char c : str) {
+        a.push_back(mk_vm_simple(c));
     }
-    return r;
+    return mk_vm_constructor(2, mk_vm_simple(str.size()), to_obj(a));
 }
 }
