library/init/data/string/lemmas.lean
@@ -5,6 +5,7 @@ Author: Leonardo de Moura
 -/
 prelude
 import init.meta
+import init.data.array.lemmas
 
 namespace string
 lemma empty_ne_str (c : char) (s : string) : empty ≠ str s c :=
@@ -14,8 +15,31 @@ lemma str_ne_empty (c : char) (s : string) : str s c ≠ empty :=
 begin cases s, unfold str empty, intro h, injection h, contradiction end
 
 lemma str_ne_str_left {c₁ c₂ : char} (s₁ s₂ : string) : c₁ ≠ c₂ → str s₁ c₁ ≠ str s₂ c₂ :=
-begin cases s₁, cases s₂, intros h₁ h₂, unfold str at h₂, injection h₂ with h, injection h, contradiction end
+begin
+  cases s₁ with n₁ a₁,
+  cases s₂ with n₂ a₂,
+  unfold str,
+  intros h₁ h₂,
+  injection h₂ with h₂₁ h₂₂,
+  injection h₂₁,
+  subst n₂,
+  have: a₁.push_back c₁ = a₂.push_back c₂, from eq_of_heq h₂₂,
+  have: c₁ = c₂, from array.push_back_inj_right this,
+  contradiction
+end
 
 lemma str_ne_str_right (c₁ c₂ : char) {s₁ s₂ : string} : s₁ ≠ s₂ → str s₁ c₁ ≠ str s₂ c₂ :=
-begin cases s₁, cases s₂, intros h₁ h₂, unfold str at h₂, injection h₂ with h, injection h, subst data, contradiction end
+begin
+  cases s₁ with n₁ a₁,
+  cases s₂ with n₂ a₂,
+  unfold str,
+  intros h₁ h₂,
+  injection h₂ with h₂₁ h₂₂,
+  injection h₂₁,
+  subst n₂,
+  have: a₁.push_back c₁ = a₂.push_back c₂, from eq_of_heq h₂₂,
+  have: a₁ = a₂, from array.push_back_inj_left this,
+  subst a₁,
+  contradiction
+end
 end string
